ordered.v
@@ -6,11 +6,41 @@ Inductive ordered : list nat -> Prop :=
 	onl : ordered []
   | oss : forall x : nat, ordered [x]
   | ocn : forall (x y : nat) (l : list nat),
-         ordered (y :: l) -> x <= y -> ordered (x :: y :: l)
-.
+         ordered (y :: l) -> x <= y -> ordered (x :: y :: l).
+
+(* the following is the bugged version*)
+Inductive ordered_bad : list nat -> Prop :=
+   onlb : ordered_bad []
+  | ossb : forall x : nat, ordered_bad [x]
+  | ocnb : forall (x y : nat) (l : list nat),
+                ordered_bad l  -> x <= y -> ordered_bad (x:: y :: l).         
+Hint  Constructors ordered.
+Goal ordered [1;2;3;4;5;5;12;13].
+auto 20.
+Qed.
+
+
+Inductive insert (x : nat) : list nat -> list nat -> Prop:=
+ | inil: insert  x [] [x]
+ |ic1 : forall y ys, x <= y -> insert x (y :: ys) (x :: y :: ys)
+ |ic2: forall y ys ns, y < x -> insert x ys ns ->  insert x (y :: ys) (y :: ns).
+
+ Hint  Constructors insert.
+ Goal exists L, insert 3 ( 1 :: 2 :: nil) L.
+ eauto 10.
+  Qed.
+  
+  Conjecture pres: forall x xs ys, ordered ys -> insert x xs ys -> ordered ys.
+  
 Elpi Command pbt.
 Elpi Accumulate File "pbt/src/kernel.mod".
+Elpi Accumulate File "pbt/src/fpc-qbound.mod".
 Elpi Typecheck.
+
+Elpi Query lp:{{
+  interp {{ 1 <= 2}}.
+  }}.
+
 Fail Elpi Query lp:{{
   interp {{ordered [1;0;2].}}.
   }}.
@@ -20,9 +50,64 @@ Elpi Query lp:{{
   }}.
 
 Elpi Query lp:{{
-coq.locate "le" (indt LE), coq.env.indt LE _ _ _ T C Ts.
+  not (interp {{ordered [1;0;2].}}).
+  }}.
+
+Elpi Query lp:{{
+  interp {{ 1 <= 22}}.
+  }}.
+
+Elpi Query lp:{{
+  interp {{ 1 = 1}}.
+  }}.
+
+(* we don't do reflexivity yet*)
+Fail Elpi Query lp:{{
+  interp {{ 1 = (0 + 1)}}.
+  }}.
+
+(* comparison with auto*)
+Goal 1 <= (22 + 1).
+simpl.
+auto 25.
+Qed.
+ 
+  (* auto here fails without the right bound, but vanilla has no problem*)  
+    Goal
+    True /\ True /\ True /\ True /\ True /\ True.
+  Proof.
+    auto.
+    Restart.
+    auto 6.
+  Qed.   
+
+  Elpi Query lp:{{
+  interp {{True /\ True  /\ True /\ True /\ True.}}.
+  }}.
+
+
+(* what about gvar?
+Elpi Query lp:{{
+  interp {{ordered 1 :: ?L.}}.
+  }}. *)
+
+  Elpi Query lp:{{
+	check  (qgen (qheight 4)) {{ (ordered [1;2]).}}.       
+  }}.
+
+(* 
+Elpi Query lp:{{
+coq.locate "le" (indt LE), coq.env.indt LE _ _ _  T C Ts.
 }}.
 
+
+LE: name of indictive
+T: its type
+C: list of constructors name 
+Ts list of constructors: le_n : n <= n is 
+(prod `n` (global (indt «nat»)) n \ app [global (indt «le»), n, n]) *)
+
+(*
 Elpi Query lp:{{
   coq.locate "ordered" GR,   coq.say "ordered is:" GR,
   coq.env.typeof GR Ty, coq.say "The type of ordered is:" Ty.  
@@ -32,3 +117,4 @@ Elpi Query lp:{{
     coq.locate "ordered" (indt GR),
     coq.env.indt GR _ _ _ Type Kn Types.   % get the names of the constructors
  }}.
+*)
