notes.v
@@ -1,0 +1,59 @@
+(*
+the atomic case of the interpreter:
+interp (app [global (indt Prog) | Args] as Atom)
+
+means Prog is predicate and Args are its args
+
+e.g. (le 1 2)    is 
+
+Prog = <<le>>
+Args = list of encodings of 1 and 2
+e.g. 1 is app [global (indc «S»), global (indc «O»)]
+
+Then we collect the list of constructors (the available clauses)
+and try to backchain on the atom
+
+Unclear:
+
+interp {{nat}}. 
+interp (sort _) .
+*)
+
+
+(* WHY [auto] SUCKS:
+
+ from UseAuto.v in SF:
+
+ Note that proof search tactics never perform any rewriting
+    step (tactics [rewrite], [subst]), nor any case analysis on an
+    arbitrary data structure or property (tactics [destruct] and
+    [inversion]), nor any proof by induction (tactic [induction]). So,
+    proof search is really intended to automate the final steps from
+    the various branches of a proof. It is not able to discover the
+    overall structure of a proof. 
+ 
+ The tactic [auto] is able to solve a goal that can be proved
+    using a sequence of [intros], [apply], [assumption], and [reflexivity].
+     The strategy of [auto] consists of trying all
+    of the possibilities (using a depth-first search exploration).
+ 
+    The tactic [auto] is simply defined as a shorthand for [auto 5].
+
+    The behavior of [auto n] can be summarized as follows. It first
+    tries to solve the goal using [reflexivity] and [assumption]. If
+    this fails, it tries to apply a hypothesis (or a lemma that has
+    been registered in the hint database), and this application
+    produces a number of sugoals. The tactic [auto (n-1)] is then
+    called on each of those subgoals. If all the subgoals are solved,
+    the job is completed, otherwise [auto n] tries to apply a
+    different hypothesis.
+
+    Due to its depth-first strategy, eauto can get exponentially slower as the 
+    depth search increases, even when a short proof exists. 
+    In general, to make proof search run reasonably fast, one should avoid 
+    using a depth search greater than 5 or 6. 
+    
+     [auto ]cannot exploit lemmas whose instantiation cannot be directly deduced 
+     from the proof goal (typically where there is an essentially exsitentuial variable, 
+     and we ween to move to the more expensive [eauto]
+    *)
