rev.v
@@ -1,0 +1,41 @@
+From elpi Require Import elpi.
+Require Import Arith List. Import ListNotations.
+Require Import Coq.Lists.List.
+
+Inductive append : list nat -> list nat -> list nat -> Prop :=
+
+anl : forall xs, append [] xs xs
+|acn: forall xs ys zs x, 
+append xs ys zs -> append (x :: xs) ys (x :: zs).
+
+Hint Constructors append.
+Goal append [1;2] [3;4] [1;2;3;4].
+auto.
+Qed.
+
+Elpi Command pbt.
+Elpi Accumulate File "pbt/src/kernel.mod".
+Elpi Typecheck.
+Elpi Query lp:{{
+  interp {{append [1;2] [3;4] [1;2;3;4].}}.
+  }}.
+
+Inductive rev : list nat -> list nat -> Prop :=
+r1nl : rev [] []
+| r1c : forall (x: nat) (l ts rs : list nat),
+       rev l ts -> append ts [x] rs -> rev (x  :: l) rs.
+
+Elpi Query lp:{{
+        interp {{rev  [1;2] [2;1].}}.
+        }}.       
+(* iterative*)
+Inductive revA : list nat -> list nat -> list nat -> Prop :=
+rnl : forall acc, revA [] acc acc
+| rc : forall (x: nat) (l acc rs : list nat),
+       revA l (x :: acc) rs  -> revA (x  :: l) (x :: acc) rs.
+
+Inductive rev2 : list nat -> list nat -> Prop :=
+r: forall xs ys, revA xs [] ys -> rev2 xs ys.
+
+Goal rev ([1;2]) ([2;1]).
+Abort.
